theories/TM/Code/List/App.v
@@ -1,0 +1,248 @@
+From Undecidability Require Import ProgrammingTools.
+From Undecidability Require Import CaseNat CaseList CaseSum. (* [TM.Code.CaseSum] contains [Constr_Some] and [Constr_None]. *)
+
+Local Arguments skipn { A } !n !l.
+Local Arguments plus : simpl never.
+Local Arguments mult : simpl never.
+
+ 
+Local Arguments Encode_list : simpl never.
+Local Arguments Encode_nat : simpl never.
+
+Set Default Proof Using "Type".
+
+
+From Undecidability Require Import TM.Basic.Mono TM.Code.Copy.
+
+
+
+Lemma pair_eq (A B : Type) (a1 a2 : A) (b1 b2 : B) :
+  (a1, b1) = (a2, b2) ->
+  a1 = a2 /\ b1 = b2.
+Proof. intros H. now inv H. Qed.
+
+
+Section ListStuff.
+  Variable X : Type.
+
+  (* TODO: -> base *)
+  Lemma app_or_nil (xs : list X) :
+    xs = nil \/ exists ys y, xs = ys ++ [y].
+  Proof.
+    induction xs as [ | x xs IH]; cbn in *.
+    - now left.
+    - destruct IH as [ -> | (ys&y&->) ].
+      + right. exists nil, x. cbn. reflexivity.
+      + right. exists (x :: ys), y. cbn. reflexivity.
+  Qed.
+
+  (* TODO: -> base *)
+  Lemma map_removelast (A B : Type) (f : A -> B) (l : list A) :
+    map f (removelast l) = removelast (map f l).
+  Proof.
+    induction l as [ | a l IH]; cbn in *; auto.
+    destruct l as [ | a' l]; cbn in *; auto.
+    f_equal. auto.
+  Qed.
+
+  (* TODO: -> base *)
+  Corollary removelast_app_singleton (xs : list X) (x : X) :
+    removelast (xs ++ [x]) = xs.
+  Proof. destruct xs. reflexivity. rewrite removelast_app. cbn. rewrite app_nil_r. reflexivity. congruence. Qed.
+
+  (* TODO: -> base *)
+  Corollary removelast_cons (xs : list X) (x : X) :
+    xs <> nil ->
+    removelast (x :: xs) = x :: removelast xs.
+  Proof. intros. change (x :: xs) with ([x] ++ xs). now rewrite removelast_app. Qed.
+
+
+  (* TODO: -> base *)
+  Corollary removelast_length (xs : list X) :
+    length (removelast xs) = length xs - 1.
+  Proof.
+    destruct (app_or_nil xs) as [ -> | (x&xs'&->)].
+    - cbn. reflexivity.
+    - rewrite removelast_app_singleton. rewrite app_length. cbn. lia.
+  Qed.
+
+End ListStuff.
+
+
+(** ** Append *)
+
+(** I simply copy memory instead of using constructors/deconstructors. The former approach is maybe easier, but I want to use fewer internal tapes. *)
+Section Append.
+
+  Variable (sigX : finType) (X : Type) (cX : codable sigX X).
+  Hypothesis (defX: inhabitedC sigX).
+
+  Notation sigList := (FinType (EqType (sigList sigX))) (only parsing).
+
+  Let stop : sigList^+ -> bool :=
+    fun x => match x with
+          | inl (START) => true (* halt at the start symbol *)
+          | _ => false
+          end.
+
+  Definition App'_size {sigX X : Type} {cX : codable sigX X} (xs : list X) (s1 : nat) := s1 - (size (Encode_list cX) xs - 1).
+
+  Definition App'_Rel : Rel (tapes sigList^+ 2) (unit * tapes sigList^+ 2) :=
+    ignoreParam (fun tin tout =>
+                   forall (xs ys : list X) (s0 s1 : nat),
+                     tin[@Fin0] ≃(;s0) xs ->
+                     tin[@Fin1] ≃(;s1) ys ->
+                     tout[@Fin0] ≃(;s0) xs /\
+                     tout[@Fin1] ≃(;App'_size xs s1) xs ++ ys).
+
+
+  Definition App' : pTM sigList^+ unit 2 :=
+    LiftTapes (MoveRight _;; Move Lmove;; Move Lmove) [|Fin0|];;
+    CopySymbols_L stop.
+
+  Lemma App'_Realise : App' ⊨ App'_Rel.
+  Proof.
+    eapply Realise_monotone.
+    { unfold App'. TM_Correct.
+      - apply MoveRight_Realise with (X := list X).
+    }
+    {
+      intros tin ((), tout) H. cbn. intros xs ys s0 s1 HEncXs HEncYs.
+      destruct HEncXs as (ls1&HEncXs&Hs0), HEncYs as (ls2&HEncYs&Hs1). TMSimp; clear_trivial_eqs.
+      rename H into HMoveRight; rename H0 into HCopy.
+      modpon HMoveRight. repeat econstructor. destruct HMoveRight as (ls3&HEncXs'). TMSimp.
+      unfold App'_size in *.
+
+      pose proof app_or_nil xs as [ -> | (xs'&x&->) ]; cbn in *; auto.
+      - rewrite CopySymbols_L_Fun_equation in HCopy; cbn in *. inv HCopy; TMSimp. repeat econstructor.
+        + lia.
+        + rewrite Encode_list_hasSize. cbn. lia.
+      - cbv [Encode_list] in *; cbn in *.
+        rewrite encode_list_app in HCopy. cbn in *.
+        rewrite !map_rev, !map_map, <- map_rev in HCopy.
+
+        rewrite rev_app_distr in HCopy. rewrite <- tl_rev in HCopy. rewrite map_app, <- !app_assoc in HCopy.
+        rewrite <- tl_map in HCopy. rewrite map_rev in HCopy. cbn in *. rewrite <- app_assoc in HCopy. cbn in *.
+        rewrite !List.map_app, !List.map_map in HCopy. rewrite rev_app_distr in HCopy. cbn in *.
+        rewrite map_rev, tl_rev in HCopy.
+
+        rewrite app_comm_cons, app_assoc in HCopy. rewrite CopySymbols_L_correct_moveleft in HCopy; cbn in *; auto.
+        + rewrite rev_app_distr, rev_involutive, <- app_assoc in HCopy. inv HCopy; TMSimp.
+          * rewrite <- app_assoc. cbn. repeat econstructor.
+            -- f_equal. cbn. rewrite encode_list_app. rewrite map_map, map_app, <- app_assoc.
+               cbn.
+               f_equal.
+               ++ now rewrite rev_involutive, map_removelast.
+               ++ f_equal. now rewrite map_app, List.map_map, <- app_assoc.
+            -- lia.
+            -- f_equal. cbn. rewrite rev_involutive, <- !app_assoc, !map_map. rewrite !encode_list_app. rewrite map_app, <- app_assoc.
+               rewrite <- map_removelast. f_equal. cbn [encode_list].
+               rewrite removelast_cons by (intros (?&?) % appendNil; congruence).
+               cbn. f_equal.
+               rewrite !map_app, <- !app_assoc.
+               rewrite !removelast_app by congruence.
+               now rewrite !map_app, <- !app_assoc, !map_map.
+            -- simpl_list. rewrite encode_list_app. rewrite skipn_length. cbn. simpl_list. rewrite removelast_length. cbn. simpl_list. simpl_list. rewrite removelast_length. cbn. lia.
+        + cbn.
+          intros ? [ (?&<-&?) % in_rev % in_map_iff | H' % in_rev ] % in_app_iff. cbn. auto. cbn in *.
+          rewrite rev_involutive, <- map_removelast in H'.
+          apply in_app_iff in H' as [ (?&<-&?) % in_map_iff | [ <- | [] ] ]. all: auto.
+    }
+  Qed.
+
+
+
+  Definition App'_steps {sigX X : Type} {cX : codable sigX X} (xs : list X) :=
+    29 + 12 * size _ xs.
+
+  Definition App'_T : tRel sigList^+ 2 :=
+    fun tin k => exists (xs ys : list X), tin[@Fin0] ≃ xs /\ tin[@Fin1] ≃ ys /\ App'_steps xs <= k.
+
+  Lemma App'_Terminates : projT1 App' ↓ App'_T.
+  Proof.
+    eapply TerminatesIn_monotone.
+    { unfold App'. TM_Correct. (* This is a bit strange, because [App'] is a sequence of two sequences. *)
+      - apply MoveRight_Realise with (X := list X).
+      - apply MoveRight_Realise with (X := list X).
+      - apply MoveRight_Terminates with (X := list X).
+    }
+    {
+      intros tin k (xs&ys&HEncXS&HEncYs&Hk). unfold App'_steps in *.
+      exists (12+4*size _ xs), (16+8*size _ xs). repeat split; cbn; try lia.
+      exists (8+4*size _ xs), 3. repeat split; cbn; try lia. eauto.
+      intros tmid1 () H. modpon H.
+      exists 1, 1. repeat split; try lia. eauto.
+      intros tmid (). intros H; TMSimp; clear_trivial_eqs. modpon H.
+      destruct H as (ls&HEncXs); TMSimp.
+      cbv [Encode_list]; cbn in *.
+
+      destruct (app_or_nil xs) as [-> | (xs'&x&->)]; cbn in *.
+      { (* [xs = nil] *)
+        rewrite CopySymbols_L_steps_equation. cbn. lia.
+      }
+      { (* [xs = xs' ++ [x]] *)
+        rewrite encode_list_app.
+        rewrite map_rev, map_map, <- map_rev.
+        rewrite rev_app_distr. cbn. rewrite <- app_assoc, rev_app_distr, <- app_assoc. cbn.
+        rewrite CopySymbols_L_steps_moveleft; cbn; auto.
+        rewrite map_length, !app_length, rev_length. cbn. rewrite map_length, rev_length, !app_length, !map_length. cbn.
+        rewrite removelast_length. lia.
+      }
+    }
+  Qed.
+
+
+  Definition App : pTM sigList^+ unit 3 :=
+    LiftTapes (CopyValue _) [|Fin1; Fin2|];;
+    LiftTapes (App') [|Fin0; Fin2|].
+
+
+  (*
+  Lemma App_Computes : App ⊨ Computes2_Rel (@app X).
+  Proof.
+    eapply Realise_monotone.
+    { unfold App. TM_Correct.
+      - apply CopyValue_Realise with (X := list X).
+      - apply App'_Realise.
+    }
+    {
+      intros tin ((), tout) H. cbn. intros xs ys HEncXs HEncYs HOut _.
+      TMSimp. rename H into HCopy; rename H0 into HComp.
+      modpon HCopy. modpon HComp.
+      repeat split; auto.
+      - intros i; destruct_fin i.
+    }
+  Qed.
+*)
+
+
+  Definition App_steps {sigX X : Type} {cX : codable sigX X} (xs ys : list X) :=
+    55 + 12 * size _ xs + 12 * size _ ys.
+
+
+  Definition App_T : tRel sigList^+ 3 :=
+    fun tin k => exists (xs ys : list X), tin[@Fin0] ≃ xs /\ tin[@Fin1] ≃ ys /\ isVoid tin[@Fin2] /\ App_steps xs ys <= k.
+
+  Lemma App_Terminates : projT1 App ↓ App_T.
+  Proof.
+    eapply TerminatesIn_monotone.
+    { unfold App. TM_Correct.
+      - apply CopyValue_Realise with (X := list X).
+      - apply CopyValue_Terminates with (X := list X).
+      - apply App'_Terminates.
+    }
+    {
+      intros tin k (xs&ys&HEncXs&HEnYs&HRigh2&Hk).
+      exists (25 + 12 * size _ ys), (App'_steps xs). repeat split; cbn; eauto.
+      unfold App'_steps, App_steps in *. lia.
+      intros tmid () (HApp'&HInjApp'); TMSimp. modpon HApp'.
+      hnf. cbn. do 2 eexists. repeat split; eauto.
+    }
+  Qed.
+
+End Append.
+
+
+Arguments App'_steps {sigX X cX} : simpl never.
+Arguments App'_size {sigX X cX} : simpl never.
+
