theories/TM/Code/List/Cons_constant.v
@@ -1,0 +1,71 @@
+From Undecidability Require Import ProgrammingTools.
+From Undecidability Require Import CaseList WriteString. 
+
+Module Cons_constant.
+Section Fix.
+
+  Context {Σ__X: finType} {X : Type} {cX : codable Σ__X X}.
+
+  
+  (* Local Instance retr_X : Retract Σ__X Σ := (Retract_sigList_X _). *)
+
+  Variable (c:X).
+
+  Definition M : pTM (sigList Σ__X)^+ unit 1 :=
+      WriteString Lmove (rev (inr sigList_cons::map (fun x => inr (sigList_X x)) ((encode c))));;
+      Move Lmove;;
+      Write (inl START).
+
+  Definition Rel : pRel (sigList Σ__X)^+ unit 1 :=
+    ignoreParam (
+        fun tin tout =>
+          forall l (s0 : nat),
+            tin[@Fin0] ≃(;s0) l ->
+            tout[@Fin0] ≃(;s0 - size _ c - 1) c :: l
+    ).
+
+  
+  Lemma Realises : M ⊨ Rel.
+  Proof.
+    eapply Realise_monotone.
+    { unfold M. TM_Correct. eapply RealiseIn_Realise,WriteString_Sem. }
+    {
+      intros tin ((), tout) H. TMSimp.
+      destruct H2 as (?&->&?);cbn.
+      simpl_tape.
+      rewrite WriteString_L_left;cbn. autorewrite with list.
+      erewrite !tape_right_move_left. 
+      2:{rewrite WriteString_L_current. autorewrite with list. cbn. reflexivity. }   
+      rewrite WriteString_L_right. cbn.
+      eexists. repeat (cbn;autorewrite with list;try rewrite !map_map).
+      split. reflexivity.
+      rewrite tl_length,List.skipn_length. unfold size. nia.
+    }
+  Qed.
+
+  Definition time {sigX X : Type} {cX : codable sigX X} := 5 + 2 * size _ c.
+
+  Lemma Terminates :
+    projT1 M ↓
+           (fun tin k =>
+              exists (l: list X) ,
+                tin[@Fin0] ≃ l /\
+                time <= k).
+  Proof.
+    unfold Constr_cons_steps. eapply TerminatesIn_monotone.
+    { unfold M. TM_Correct.
+      eapply RealiseIn_Realise. 2:eapply RealiseIn_TerminatesIn.
+      all:apply WriteString_Sem.
+    }
+    {
+      intros tin k (l&Hin&Hk). cbn. autorewrite with list.
+      infTer 4.
+      2:{
+        intros. infTer 4. intros. reflexivity.   
+      }
+      cbn. unfold time,size in Hk. nia.
+    } 
+  Qed.
+
+End Fix.  
+End Cons_constant.
