theories/TM/Code/List/Nth.v
@@ -1,0 +1,267 @@
+From Undecidability Require Import ProgrammingTools Hoare.
+From Undecidability Require Import CaseNat CaseList CaseSum. (* [TM.Code.CaseSum] contains [Constr_Some] and [Constr_None]. *)
+
+
+Local Arguments skipn { A } !n !l.
+Local Arguments plus : simpl never.
+Local Arguments mult : simpl never.
+
+ 
+Local Arguments Encode_list : simpl never.
+Local Arguments Encode_nat : simpl never.
+
+Set Default Proof Using "Type".
+
+(** ** Other Implementation of [nth_error] *)
+
+Section Nth'.
+
+  (** In this implementation of [nth_error], instead of encoding an option to the output tape, we use the finite parameter to indicate whether the result is [Some] or [None]. The advantage is that the client doesn't have to add the option to its alphabet. *)
+
+  Variable (sig sigX : finType) (X : Type) (cX : codable sigX X).
+  (* Hypothesis (defX: inhabitedC sigX). *)
+
+  Variable (retr1 : Retract (sigList sigX) sig) (retr2 : Retract sigNat sig).
+  Local Instance retr_X_list' : Retract sigX sig := ComposeRetract retr1 (Retract_sigList_X _).
+
+  (* Check _ : codable sig (list X). *)
+  (* Check _ : codable sig nat. *)
+
+  Definition Nth'_Step_size {sigX X : Type} {cX : codable sigX X} (n : nat) (l : list X) : Vector.t (nat -> nat) 3 :=
+    match n, l with
+    | S n', x :: l' =>
+      [| CaseList_size0 x; S; CaseList_size1 x >> Reset_size x|]
+    | 0, x :: x' =>
+      [|fun s0 => CaseList_size0 x s0; id; fun s2 => CaseList_size1 x s2|]
+    | 0, nil => [|id; id; id|]
+    | S n', nil => [|id; fun s1 => S s1; id|]
+    end.
+
+  Definition Nth'_Step : pTM sig^+ (option bool) 3 :=
+    If (LiftTapes (ChangeAlphabet CaseNat _) [|Fin1|])
+       (If (LiftTapes (ChangeAlphabet (CaseList sigX) _) [|Fin0; Fin2|]) (* n = S n' *)
+           (Return (LiftTapes (Reset _) [|Fin2|]) None) (* l = x :: l'; continue *)
+           (Return Nop (Some false))) (* l = nil; return false *)
+       (Relabel (LiftTapes (ChangeAlphabet (CaseList sigX) _) [|Fin0; Fin2|]) Some) (* n = 0 *)
+  .
+
+
+  Definition Nth'_Step_steps {sigX X : Type} {cX : codable sigX X} (l : list X) (n : nat) :=
+    match n, l with
+    | S n', x :: l' =>
+      2 + CaseNat_steps + CaseList_steps_cons x + Reset_steps x
+    | S n', nil =>
+      2 + CaseNat_steps + CaseList_steps_nil
+    | O, x :: l' =>
+      1 + CaseNat_steps + CaseList_steps_cons x
+    | O, nil =>
+      1 + CaseNat_steps + CaseList_steps_nil
+    end.
+
+    Definition Nth'_Step_steps_CaseList (xs : list X) :=
+      match xs with
+      | x :: xs' => 1 + CaseList_steps_cons x + Reset_steps x
+      | nil => 1 + CaseList_steps_nil
+      end.
+  
+    Lemma Nth'_Step_SpecT_size (n : nat) (xs : list X) (ss : Vector.t nat 3) :
+      TripleT
+        (tspec (withSpace (SpecVector [|Contains _ xs; Contains _ n; Void|]) ss))
+        (Nth'_Step_steps xs n) Nth'_Step
+        (fun yout =>
+           tspec (withSpace
+                    match yout, n, xs with
+                    | None,       S n', x::xs' => SpecVector [|Contains _ xs'; Contains _ n'; Void|]
+                    | Some true,     0, x::xs' => SpecVector [|Contains _ xs'; Contains _ 0;  Contains _ x|]
+                    | Some false,    O,   nil => SpecVector [|Contains _ nil; Contains _ 0;  Void|]
+                    | Some false, S n',   nil => SpecVector [|Contains _ nil; Contains _ n'; Void|]
+                    | _, _, _ => SpecFalse
+                    end (appSize (Nth'_Step_size n xs) ss))).
+    Proof.
+      start_TM.
+      unfold Nth'_Step.
+      eapply If_SpecT with (k1 := CaseNat_steps) (k2 := Nth'_Step_steps_CaseList xs) (k3 := CaseList_steps xs).
+      - hstep; cbn.
+        hstep; cbn. (* or [eapply ChangeAlphabet_SpecT_space_pre.] *)
+        hstep; cbn. cbn. tspec_ext.
+      - cbn. destruct n as [ | n']; cbn in *; auto.
+        (** Like in the Realisation proof, we make a case-distinction over the value of [xs]. *)
+        destruct xs as [ | x xs']; cbn in *; auto.
+        + eapply If_SpecT with (k2 := 0).
+          * hstep; cbn. hstep; cbn. hstep; cbn. cbn. tspec_ext.
+          * cbn. auto. (* The "Then" case of the "If CaseList". We are not in this state, since [xs=nil]. *)
+          * cbn. hstep; cbn. hstep; cbn. cbn. intros _. tspec_ext.
+          * cbn. intros tin yout tout. destruct yout; cbn in *; auto.
+        + eapply If_SpecT.
+          * hstep; cbn. hstep; cbn. hstep; cbn. cbn. tspec_ext.
+          * cbn. hstep; cbn. hstep; cbn. apply Reset_SpecT_space. cbn. intros _. tspec_ext.
+          * cbn. auto. (* The "Else" case of the "If CaseList". We are not in this state, since [xs=x::xs']. *)
+          * cbn. intros tin yout tout. destruct yout; cbn in *; auto.
+      - cbn. destruct n as [ | n']; cbn in *; auto.
+        hstep; cbn. hstep; cbn. hstep; cbn. hstep; cbn.
+        cbn. tspec_ext.
+        intros yout tout. destruct yout, xs as [ | x xs']; cbn in *; auto.
+        + intros. tspec_ext.
+        + intros. tspec_ext.
+      - intros ? ? ? ? ?. destruct yout, n as [ | n'], xs as [ | x xs']; cbn in *; auto.
+    Qed.
+
+  Fixpoint Nth'_Loop_size {sigX X : Type} {cX : codable sigX X} (n : nat) (l : list X) {struct n} : Vector.t (nat -> nat) 3 :=
+    match n, l with
+    | S n', x :: l' => Nth'_Step_size n l >>> Nth'_Loop_size n' l'
+    | _, _ => Nth'_Step_size n l
+    end.
+
+  Definition Nth'_Loop := While Nth'_Step.
+
+  Fixpoint Nth'_Loop_steps {sigX X : Type} {cX : codable sigX X} (l : list X) (n : nat) { struct l } :=
+    match n, l with
+    | S n', x :: l'  => S (Nth'_Step_steps l n) + Nth'_Loop_steps l' n' (* continue *)
+    | S n', nil => Nth'_Step_steps l n (* return *)
+    | O, x :: l' => Nth'_Step_steps l n (* return *)
+    | O, nil => Nth'_Step_steps l n (* only [CaseNat] and [If] *)
+    end.
+
+    Lemma Nth'_Loop_SpecT_size xs n (ss : Vector.t nat 3) :
+    TripleT
+      (tspec (withSpace (SpecVector [|Contains _ xs; Contains _ n; Void|]) ss))
+      (Nth'_Loop_steps xs n) Nth'_Loop
+      (fun yout =>
+         tspec
+           (withSpace
+              match yout, nth_error xs n with
+              | true, Some x => SpecVector [|Contains _ (skipn (S n) xs); Contains _ (n - (S (length xs))); Contains _ x|]
+              | false, None  => SpecVector [|Contains _ (skipn (S n) xs); Contains _ (n - (S (length xs))); Void|]
+              | _, _ => SpecFalse
+              end
+              (appSize (Nth'_Loop_size n xs) ss))).
+  Proof.
+    eapply While_SpecT with (P := fun '(xs,n,ss) => _) (Q := fun '(xs,n,ss) => _) (R := fun '(xs,n,ss) => _) (g := fun '(xs,n,ss) => _) (f := fun '(xs,n,ss) => _) (x := (xs,n,ss));
+      clear xs n ss; intros ((xs,n),ss).
+    - apply Nth'_Step_SpecT_size.
+    - cbn. intros yout tmid tout H1 H2.
+      destruct yout, n as [ | n'], xs as [ | x xs']; cbn in *; auto.
+      replace (n' - 0) with n' by lia. auto.
+    - cbn. intros yout tmid tout H1.
+      destruct n as [ | n'], xs as [ | x xs']; cbn in *; auto.
+      eexists (xs', n', _). repeat split; cbn.
+      + eauto.
+      + reflexivity.
+      + eauto.
+  Qed.
+
+
+  (** We don't want to save, but reset, [n]. *)
+  Definition Nth' : pTM sig^+ bool 4 :=
+    LiftTapes (CopyValue _) [|Fin0; Fin3|];; (* Save l (on t0) to t3 *)
+    If (LiftTapes (Nth'_Loop) [|Fin3; Fin1; Fin2|]) (* Execute the loop with the copy of l *)
+       (Return (LiftTapes (Reset _) [|Fin3|];; (* Reset the copy of [l] *)
+                LiftTapes (Reset _) [|Fin1|] (* Reset [n] *)
+               ) true)
+       (Return (LiftTapes (Reset _) [|Fin3|];; (* Reset the copy of [l] *)
+                LiftTapes (Reset _) [|Fin1|] (* Reset [n] *)
+               ) false)
+  .
+
+  Definition Nth'_size {sigX X : Type} {cX : codable sigX X} (l : list X) (n : nat) :=
+    [| id;
+       (Nth'_Loop_size n l)[@Fin1] >> Reset_size (n - (S (length l)));
+       (Nth'_Loop_size n l)[@Fin2];
+       CopyValue_size l >> (Nth'_Loop_size n l)[@Fin0] >> Reset_size (skipn (S n) l)
+     |].
+
+     
+  Definition Nth'_steps {sigX X : Type} {cX : codable sigX X} (l : list X) (n : nat) :=
+    3 + CopyValue_steps l + Nth'_Loop_steps l n + Reset_steps (skipn (S n) l) + Reset_steps (n - S (length l)).
+
+
+     
+  Lemma Nth'_SpecT_size (xs : list X) (n : nat) (ss : Vector.t nat 4) :
+    TripleT
+      (tspec (withSpace (SpecVector [|Contains _ xs; Contains _ n; Void; Void|]) ss))
+      (Nth'_steps xs n) Nth'
+      (fun yout =>
+        tspec (withSpace
+                  match yout, nth_error xs n with
+                  | true, Some x => SpecVector [|Contains _ xs; Void; Contains _ x; Void|]
+                  | false, None => SpecVector [|Contains _ xs; Void; Void; Void|]
+                  | _, _ => SpecFalse
+                  end (appSize (Nth'_size xs n) ss))).
+  Proof.
+    start_TM.
+    unfold Nth'.
+    hstep; cbn. hstep; cbn. apply CopyValue_SpecT_size.
+    cbn. intros _. eapply If_SpecT; cbn.
+    - hstep; cbn. eapply ConsequenceT_pre. apply Nth'_Loop_SpecT_size. tspec_ext. reflexivity.
+    - cbn. destruct (nth_error xs n) as [ x | ]; cbn in *; auto.
+      hstep; cbn. hstep; cbn. hstep; cbn. apply Reset_SpecT_space with (X := list X).
+      cbn. intros []. eauto. hstep; cbn. apply Reset_SpecT_space with (X := nat). reflexivity.
+      cbn. intros _. auto.
+    - cbn. destruct (nth_error xs n) as [ x | ]; cbn in *; auto.
+      hstep; cbn. hstep; cbn. hstep; cbn. apply Reset_SpecT_space with (X := list X).
+      cbn. intros []. eauto. hstep; cbn. apply Reset_SpecT_space with (X := nat). reflexivity.
+      cbn. intros _. auto.
+    - cbn. intros tin yout tout ? ?. cbn. destruct yout; cbn in *; auto.
+    - unfold Nth'_steps. cbn. lia.
+  Qed.
+
+
+  Section Legacy.
+    
+    Definition Nth'_Rel : pRel sig^+ bool 4 :=
+      fun tin '(yout, tout) =>
+        forall (l : list X) (n : nat) s0 s1 s2 s3,
+          tin[@Fin0] ≃(;s0) l ->
+          tin[@Fin1] ≃(;s1) n ->
+          isVoid_size tin[@Fin2] s2 ->
+          isVoid_size tin[@Fin3] s3 ->
+          match yout with
+          | true =>
+            exists (x : X),
+            nth_error l n = Some x /\
+            tout[@Fin0] ≃(;(Nth'_size l n)[@Fin0]s0) l /\
+            isVoid_size tout[@Fin1] ((Nth'_size l n)[@Fin1]s1) /\
+            tout[@Fin2] ≃(;(Nth'_size l n)[@Fin2]s2) x /\
+            isVoid_size tout[@Fin3] ((Nth'_size l n)[@Fin3]s3)
+          | false =>
+            nth_error l n = None /\
+            tout[@Fin0] ≃(;(Nth'_size l n)[@Fin0]s0) l /\
+            isVoid_size tout[@Fin1] ((Nth'_size l n)[@Fin1]s1) /\
+            isVoid_size tout[@Fin2] ((Nth'_size l n)[@Fin2]s2) /\
+            isVoid_size tout[@Fin3] ((Nth'_size l n)[@Fin3]s3)
+          end.
+
+    Lemma Nth'_Realise : Nth' ⊨ Nth'_Rel.
+    Proof.
+      repeat (eapply RealiseIntroAll;intro). eapply Realise_monotone.
+      -eapply TripleT_Realise. eapply Nth'_SpecT_size with (ss:=[|_;_;_;_|]).
+      -unfold Nth'_Rel. intros ? [] H **. modpon H.
+      {unfold "≃≃",withSpace;cbn. intros i; destruct_fin i;cbn. exact H3. all:eassumption. }
+      repeat destruct _;unfold "≃≃",withSpace in H;cbn in H.
+      2,3:contradiction.
+      all:specializeFin H;eauto 6.
+    Qed.
+
+
+    Definition Nth'_T : tRel sig^+ 4 :=
+      fun tin k => exists (l : list X) (n : nat),
+          tin[@Fin0] ≃ l /\
+          tin[@Fin1] ≃ n /\
+          isVoid tin[@Fin2] /\ isVoid tin[@Fin3] /\
+          Nth'_steps l n <= k.
+
+    Lemma Nth'_Terminates : projT1 Nth' ↓ Nth'_T.
+    Proof.
+      repeat (eapply TerminatesInIntroEx;intro). eapply TerminatesIn_monotone.
+      -eapply TripleT_TerminatesIn. eapply TripleT_RemoveSpace,Nth'_SpecT_size.
+      -intros ? k H **. modpon H.
+      split. 2:eassumption. 
+      unfold "≃≃",withSpace;cbn. intros i; destruct_fin i;cbn. all:assumption. 
+    Qed.
+  End Legacy.
+
+End Nth'.
+
+
+Arguments Nth'_steps {sigX X cX} : simpl never.
+Arguments Nth'_size {sigX X cX} : simpl never.
