theories/TM/Code/NatSub.v
@@ -1,0 +1,42 @@
+From Undecidability Require Import TM.Code.ProgrammingTools.
+From Undecidability Require Import TM.Code.CaseNat.
+
+(* Minus x y computes x - y and returns whether x >= y (e.g., if the subtraction did not need to truncate) *)
+
+Definition Subtract_Rel : pRel (sigNat^+) bool 2 :=
+    fun tin '(b, tout) =>
+    forall (x y : nat),  
+        tin [@Fin0] ≃ x
+        -> tin [@Fin1] ≃ y
+        -> tout [@Fin0] ≃ x - y
+        /\ isVoid tout [@Fin1]
+        /\ b = (y <=? x).
+
+Definition Subtract :pTM (sigNat^+) bool 2:=
+    While (
+        If(CaseNat @ [|Fin1|])
+          (If (CaseNat @ [|Fin0|])
+              (Return Nop None)
+              (Return (Reset _ @ [|Fin1|]) (Some false)) )
+          (Return (Reset _ @ [|Fin1|]) (Some true))  
+    ).
+
+
+Lemma Subtract_Realise : Subtract ⊨ Subtract_Rel.
+Proof.
+  eapply Realise_monotone.
+  {
+    unfold Subtract. TM_Correct. all: (try (notypeclasses refine (@Reset_Realise _ _ _ _ _);shelve)).
+  }
+  {
+    apply WhileInduction.
+    - intros tin b tout [(t0_&Hif1&[Hif2|[t1_ Hif2]]) |?] x y;TMSimp;[ | ].
+      + modpon H. modpon H2. destruct y. easy. destruct x. 2:easy.
+        modpon H1. rewrite Nat.sub_0_l. cbn ["<=?"]. repeat split. contains_ext. isVoid_mono.
+      + modpon H. destruct y. 2:easy.
+        modpon H1. rewrite Nat.sub_0_r. cbn ["<=?"]. repeat split. contains_ext. isVoid_mono.
+    - intros tin tmid tout b [(t0_&Hif1&[Hif2|[t1_ Hif2]]) |?] H' x y;TMSimp;[].
+      modpon H. modpon H1. destruct x,y;try contradiction;[].
+      modpon H'. rewrite Nat.sub_succ. cbn ["<=?"]. easy.
+  } 
+Qed.
