theories/TM/Compound/WriteString.v
@@ -93,3 +93,80 @@ End Write_String.
 
 Arguments WriteString : simpl never.
 Arguments WriteString_Rel {sig} (D) (str) x y/.
+
+Lemma skipn_S (X : Type) (xs : list X) (n : nat) :
+  skipn (S n) xs = tl (skipn n xs).
+Proof.
+  revert xs. induction n as [ | n IH]; intros; cbn in *.
+  - destruct xs; auto.
+  - destruct xs; auto.
+Qed.
+
+(*
+Compute skipn 3 (tl [1;2;3;4;5;6;7]).
+Compute tl (skipn 3 [1;2;3;4;5;6;7]).
+*)
+
+Lemma skipn_tl (X : Type) (xs : list X) (n : nat) :
+  skipn n (tl xs) = tl (skipn n xs).
+Proof.
+  revert xs. induction n as [ | n IH]; intros; cbn in *.
+  - destruct xs; auto.
+  - destruct xs; cbn; auto.
+    replace (match xs with
+             | [] => []
+             | _ :: l => skipn n l
+             end)
+      with (skipn n (tl xs)); auto.
+    destruct xs; cbn; auto. apply skipn_nil.
+Qed.
+
+
+Lemma WriteString_L_local (sig : Type) (str : list sig) t :
+  str <> nil ->
+  tape_local (WriteString_Fun Lmove t str) = rev str ++ right t.
+Proof.
+  revert t. induction str as [ | s [ | s' str'] IH]; intros; cbn in *.
+  - tauto.
+  - reflexivity.
+  - rewrite IH. 2: congruence. simpl_tape. rewrite <- !app_assoc. reflexivity.
+Qed.
+
+(*
+Section Test.
+  Let t : tape nat := midtape [3;2;1] 4 [5;6;7].
+  Let str := [3;2;1].
+  Compute WriteString_Fun Lmove t str.
+  Compute (left t).
+  Compute (left (WriteString_Fun Lmove t str)).
+  Compute (skipn (length str - 1) (left t)).
+End Test.
+*)
+
+Lemma WriteString_L_left (sig : Type) (str : list sig) t :
+  left (WriteString_Fun Lmove t str) = skipn (pred (length str)) (left t).
+Proof.
+  revert t. induction str as [ | s [ | s' str'] IH]; intros; cbn -[skipn] in *.
+  - reflexivity.
+  - reflexivity.
+  - rewrite IH. simpl_tape. now rewrite skipn_S, skipn_tl.
+Qed.
+
+Lemma WriteString_L_right (sig : Type) (str : list sig) t :
+   right (WriteString_Fun Lmove t str) = tl (rev str) ++ right t.
+Proof.
+  revert t. induction str as [ | s [ | s' str'] IH]; intros; cbn in *.
+  - tauto.
+  - reflexivity.
+  - rewrite IH. simpl_tape. rewrite tl_app with (ys:=[s]),<- !app_assoc. reflexivity. intros (?&[=])%app_eq_nil.
+Qed.
+
+Lemma WriteString_L_current (sig : Type) (str : list sig) t :
+   current (WriteString_Fun Lmove t str) = hd None (map Some (rev str ++ tape_local t)).
+Proof.
+  revert t. induction str as [ | s [ | s' str'] IH]; intros; cbn in *.
+  - now destruct t.
+  - reflexivity.
+  - rewrite IH. autorewrite with list. setoid_rewrite app_assoc at 1 2.
+    rewrite !hd_app with (xs:=(map Some (rev str') ++ map Some [s'])). easy. all:intros (?&[=])%app_eq_nil.
+Qed.
